improving formatting and order

ex/exCoqRDF.v
@@ -14,41 +14,14 @@ Section Sets.
   Definition lit_t := (string * string)%type.
   Definition bn_t := nat.
 
-  (* Defining some sets for IRIs, blank nodes and literals. *)
-
-  (* Inductive Iex := *)
-  (* | isA *)
-  (* | Sonata *)
-  (* | Year. *)
-
-  Inductive B1ex :=
-  | A
-  | B
-  | C.
-
-  Inductive B2ex :=
-  | E
-  | F.
-
-  Inductive Lex :=
-  | num (n : nat).
-
 End Sets.
 
 Section Maps.
-
-  (* Defining some maps resulting in the same type domain or in another one. *)
 
   Definition mu (b : nat) : nat :=
     match b with
     | 0 => 1
     | _ => b
-    end.
-
-  Definition nu (b: nat) : B1ex :=
-    match b with
-    | 0 => A
-    | _ => B
     end.
 
 End Maps.
@@ -57,110 +30,37 @@ End Maps.
 Section Prelude.
 
   (* Transferring eqType infrastructure to the inductives *)
-
-  (* Definition eqb_i (i1 i2 : Iex) := *)
-  (*   match (i1, i2) with *)
-  (*   | (isA, isA) | (Sonata,Sonata) | (Year,Year) => true *)
-  (*   | (_,_) => false *)
-  (*   end. *)
-
-  Definition eqb_b1 (b1 b2 : B1ex) :=
-    match (b1, b2) with
-    | (A, A) | (B,B) | (C,C) => true
-    | (_,_) => false
-    end.
-
-  Definition eqb_b2 (b1 b2 : B2ex) :=
-    match (b1, b2) with
-    | (E, E) | (F,F) => true
-    | (_,_) => false
-    end.
-
-  Definition eqb_l (l1 l2 : Lex) :=
-    match (l1, l2) with
-    | ((num n), (num m)) => n == m
-    end.
-
   Lemma str_eqP : Equality.axiom String.eqb. by move=> x y; apply eqb_spec. Qed.
-  (* Lemma i_eqP : Equality.axiom eqb_i. by case; case; (try apply Bool.ReflectT=> //); apply Bool.ReflectF. Qed. *)
-  Lemma b1_eqP : Equality.axiom eqb_b1. by case; case; (try apply Bool.ReflectT=> //); apply Bool.ReflectF. Qed.
-  Lemma b2_eqP : Equality.axiom eqb_b2. by case; case; (try apply Bool.ReflectT=> //); apply Bool.ReflectF. Qed.
-  Lemma l_eqP : Equality.axiom eqb_l.
-  Proof. move=> [[|n']] [[|m']].
-         + by apply Bool.ReflectT.
-         + by apply Bool.ReflectF.
-         + by apply Bool.ReflectF.
-           apply: (iffP idP); first by rewrite /eqb_l=> /eqP ->.
-           by move=> ->; rewrite /eqb_l eqxx.
-  Qed.
 
 End Prelude.
 
-Canonical b1E := Eval hnf in EqType B1ex (EqMixin b1_eqP).
-Canonical b2E := Eval hnf in EqType B2ex (EqMixin b2_eqP).
-Canonical lE := Eval hnf in  EqType Lex (EqMixin l_eqP).
 Canonical strE := Eval hnf in EqType string (EqMixin str_eqP).
 Canonical iriE := Eval hnf in EqType iri_t (EqMixin str_eqP).
 Canonical litE := Eval hnf in [eqType of lit_t].
 
-Section TermsEx.
-
-  (* Defining some terms and testing relabeling and equality on them. *)
-
-  (* Definition I (i : Iex) {B : Type} := @Iri Iex B Lex i. *)
-  (* Definition L (l : Lex) {B : Type} := @Lit Iex B Lex l. *)
-  (* Definition Bn {B : Type} := @Bnode Iex B Lex. *)
-
-  (* Definition isA1 := @I isA B1ex. *)
-  (* Definition isA2 := @I isA B2ex. *)
-  (* Definition sonata1 := @I Sonata B1ex. *)
-  (* Definition sonata2 := @I Sonata B2ex. *)
-  (* Definition year {B : Type} := @I Year B. *)
-  (* Definition b := Bn B. *)
-  (* Definition c := Bn C. *)
-  (* Definition f := Bn F. *)
-  (* Definition n1781 {B : Type} := @L (num 1781) B. *)
-
-
-  (* Example relabeling_an_iri : (relabeling_term mu isA1) == isA1. by []. Qed. *)
-
-  (* Example relabeling_a_blank_node : (relabeling_term mu b) == c. by []. Qed. *)
-
-  (* Example relabeling_blank_node_type : (relabeling_term nu b) == f. by []. Qed. *)
-
-End TermsEx.
 Section TermsStr.
 
   (* Defining some terms and testing relabeling and equality on them. *)
-
   Definition I  := @Iri iri_t bn_t lit_t.
   Definition L  := @Lit iri_t bn_t lit_t.
   Definition Bn := @Bnode iri_t bn_t lit_t.
 
-  (* Definition isA := I "isA". *)
-  (* Definition sonata := I "sonata". *)
-  (* Definition year := I "year". *)
+  Example relabeling_an_iri :
+    (relabeling_term mu (I "isA")) == (I "isA") = true. by []. Qed.
 
-  (* Definition a := Bn A. *)
-  (* Definition z := Bn 0. *)
-  (* Definition f := Bn 5. *)
-  (* Definition n1781 {B : Type} := @L ("number","1781") B. *)
+  Example relabeling_a_blank_node :
+    (relabeling_term mu (Bn 0)) == (Bn 1) = true. by []. Qed.
 
-
-  Example relabeling_an_iri : (relabeling_term mu (I "isA")) == (I "isA") = true. by []. Qed.
-
-  Example relabeling_a_blank_node : (relabeling_term mu (Bn 0)) == (Bn 1) = true. by []. Qed.
-
-  Example relabeling_a_literal : (relabeling_term mu (L ("number","1781"))) == (I "1781") = false. by []. Qed.
+  Example relabeling_a_literal :
+    (relabeling_term mu (L ("number","1781"))) == (I "1781") = false. by []. Qed.
 
 End TermsStr.
 Section TripleStr.
 
   (* Defining some triples and testing relabeling and equality on them. *)
-
   Definition mkT := @mkTriple iri_t bn_t lit_t.
 
-  (* type aliases *)
+  (* type alias *)
   Definition tr_t := triple iri_t bn_t lit_t.
 
   Definition z_isA_sonata : tr_t. by refine (@mkT (Bn 0) (I "isA") (I "sonata") _ _). Defined.
@@ -173,9 +73,6 @@ End TripleStr.
 Section GraphStr.
   (* Defining some graphs and testing relabeling and equality on them. *)
 
-  (* type aliases *)
-  (* Definition RDF_t := rdf_graph iriE bnE litE. *)
-
   Definition OSonataG := mkRdf [:: o_isA_sonata; o_year_1781].
   Definition OSonataG_perm := mkRdf [:: o_year_1781 ; o_isA_sonata ].
   Definition ZSonataG := mkRdf [:: z_isA_sonata; o_year_1781].
@@ -186,45 +83,4 @@ Section GraphStr.
   Example graphs_prop_neq : ZSonataG == empty_rdf_graph = false. by []. Qed.
 
 End GraphStr.
-
-(* Section TripleEx. *)
-
-(*   (* Defining some triples and testing relabeling and equality on them. *) *)
-
-(*   Definition mkTriple {B : Type} := @mkTriple Iex B Lex. *)
-
-(*   (* type aliases *) *)
-(*   Definition tr_b1 := triple iE b1E lE. *)
-(*   Definition tr_b2 := triple iE b2E lE. *)
-
-(*   Definition b_isA_sonata : tr_b1. by refine (@mkTriple _ b isA1 sonata1 _ _). Defined. *)
-(*   Definition f_isA_sonata : tr_b2. by refine (@mkTriple _ f isA2 sonata2 _ _). Defined. *)
-(*   Definition c_isA_sonata : tr_b1. by refine (@mkTriple _ c isA1 sonata1 _ _). Defined. *)
-(*   Definition f_year_1781 : tr_b2. by refine (@mkTriple _ f year n1781 _ _). Defined. *)
-(*   Definition b_year_1781 : tr_b1. by refine (@mkTriple _ b year n1781 _ _). Defined. *)
-
-(*   Example relabeling_a_triple_eq : relabeling_triple mu b_isA_sonata == c_isA_sonata. by []. Qed. *)
-
-(*   Example relabeling_a_triple_neq : relabeling_triple nu b_isA_sonata == f_year_1781 = false. by []. Qed. *)
-
-(* End TripleEx. *)
-(* Section GraphEx. *)
-(*   (* Defining some graphs and testing relabeling and equality on them. *) *)
-
-(*   (* type aliases *) *)
-(*   Definition RDF_b1 := rdf_graph iE b1E lE. *)
-(*   Definition RDF_b2 := rdf_graph iE b2E lE. *)
-
-(*   Definition BSonataG : RDF_b1. by refine (@mkRdfGraph _ _ _ [:: b_isA_sonata; b_year_1781] _). Defined. *)
-(*   Definition relabeled_G : RDF_b2. by refine (@relabeling _ _ _ _ nu BSonataG _). Defined. *)
-(*   Definition BSonataG_perm : RDF_b1. by refine (@mkRdfGraph _ _ _ [:: b_year_1781 ; b_isA_sonata ] _). Defined. *)
-(*   Definition FSonataG : RDF_b2. by refine (@mkRdfGraph _ _ _ [:: f_isA_sonata; f_year_1781] _). Defined. *)
-
-(*   Example graphs_eq : eqb_rdf BSonataG BSonataG_perm. by []. Qed. *)
-(*   Example graphs_relabel_eq : eqb_rdf relabeled_G FSonataG. by []. Qed. *)
-(*   Example graphs_prop_neq : BSonataG == empty_rdf_graph = false. by []. Qed. *)
-
-(* End GraphEx. *)
-
-
 
