ex/ex.v
@@ -1,0 +1,107 @@
+From mathcomp Require Import all_ssreflect.
+Set Implicit Arguments.
+Unset Strict Implicit.
+Unset Printing Implicit Defensive.
+
+Inductive nat : Type :=
+| O
+| S : nat -> nat.
+
+Fixpoint add n m :=
+  match n with
+  | O => m
+  | S n' => add n' (S m)
+  end.
+
+Theorem addO_n : forall (n : nat), add O n = n.
+Proof. by []. Qed.
+
+Check addO_n.
+
+Fixpoint eqb_nat n m:=
+ match n,m with
+ | O,O => true
+ | S n', S m' => eqb_nat n' m'
+ | _, _ => false
+ end.
+
+Inductive opt (A : Type) :=
+| Non
+| Som : A -> opt A.
+
+ Lemma nat_eqax : Equality.axiom eqb_nat.
+ Proof. move=> n.
+ elim: n=> [| n' IHn] [| m'].
+   + by apply Bool.ReflectT.
+  + by apply Bool.ReflectF.
+  + by apply Bool.ReflectF.
+  + by move=> /=; apply: (equivP (IHn m') _); split=> [->|[->]].
+Qed.
+
+
+Definition nat_eqType := EqType nat (EqMixin nat_eqax).
+Canonical nat_eqType.
+
+Variables n m : nat.
+Check n == m.
+
+Lemma eqb_nat_trans (n m l : nat) : eqb_nat n m -> eqb_nat m l -> eqb_nat n l.
+Proof. by move/eqP=> ->. Qed.
+
+Variable is_prime : nat -> bool.
+
+Record prime : Type := mkPrime {
+  p :> nat;
+  p_prime : is_prime p
+                         }.
+
+Lemma prime_inj (p1 p2 : prime) :
+  p p1 = p p2 ->
+  p1 = p2.
+Proof. case p1; case p2=> prime1 prime1P prime2 prime2P /= eq.
+subst; congr mkPrime. 
+by apply eq_irrelevance.
+Qed.
+
+Check eq_irrelevance.
+
+Definition code (p : prime) : nat :=
+  p.
+
+Definition decode (n : nat) : option prime :=
+  if insub n : {? x | is_prime x} is Some nn
+  then Some (mkPrime (valP nn))
+  else None.
+
+Lemma pcancel_code_decode : pcancel code decode.
+Proof.
+  case=> p pP /=; rewrite /decode.
+  case: insubP => [? ? ?|].
+  by congr Some; apply prime_inj.
+  by rewrite pP.
+Qed.
+
+Definition prime_canEqMixin := PcanEqMixin pcancel_code_decode.
+
+Canonical prime_eqType :=
+  Eval hnf in EqType prime prime_canEqMixin.
+
+
+Section inj.
+
+Inductive I : Type :=
+| K.
+
+Variable p : I -> bool.
+Record r := mkR {
+  i : I;
+  iP: p i
+}.
+
+Lemma i_inj I1 I2: i I1 = i I2 ->
+  I1 = I2.
+Proof. case I1; case I2=> i1 iP1 i2 iP2 /= eq.
+subst; congr mkR. exact: eq_irrelevance.
+Qed.
+
+End inj.
